investigations/bedrock2/IncrementWait/IncrementWaitToCava.v
@@ -1,0 +1,93 @@
+Require Import Coq.Lists.List. Import ListNotations.
+Require Import Coq.ZArith.ZArith. Open Scope Z_scope.
+Require Import Coq.Strings.String. Open Scope string_scope.
+Require Import coqutil.Byte.
+Require Import coqutil.Word.Interface coqutil.Word.Properties.
+Require Import bedrock2.ZnWords.
+Require Import compiler.SeparationLogic.
+Require Import Bedrock2Experiments.RiscvMachineWithCavaDevice.ExtraRiscvMachine.
+Require Import Bedrock2Experiments.RiscvMachineWithCavaDevice.InternalMMIOMachine.
+Require Import Bedrock2Experiments.RiscvMachineWithCavaDevice.DetIncrMachine.
+Require Import Bedrock2Experiments.IncrementWait.IncrementWaitToRiscV.
+Require Import Bedrock2Experiments.IncrementWait.IncrementWaitToRiscVProperties.
+Require Import Bedrock2Experiments.RiscvMachineWithCavaDevice.Bedrock2ToCava.
+
+Definition binary: list byte := Eval compute in Pipeline.instrencode put_wait_get_asm.
+
+Definition mmioRange: word -> Prop :=
+  fun a => Constants.INCR_BASE_ADDR <= word.unsigned a < Constants.INCR_END_ADDR.
+
+Definition incr_device_state_related: IncrementWaitSemantics.state -> counter_device -> Prop.
+Admitted.
+
+Lemma initial_device_states_related:
+  incr_device_state_related IncrementWaitSemantics.IDLE device.reset_state.
+Admitted.
+
+Axiom TODO: False.
+
+Theorem IncrementWait_end2end_correct: forall p_functions p_call mH Rdata Rexec R (* <-? *)
+          (initialL: ExtraRiscvMachine counter_device) input output_placeholder sched,
+    -2^19 <= word.signed (word.sub p_functions p_call) < 2^19 ->
+    128 <= word.unsigned (word.sub stack_pastend stack_start) ->
+    word.unsigned (word.sub stack_pastend stack_start) mod 4 = 0 ->
+    word.unsigned p_functions mod 4 = 0 ->
+    word.unsigned p_call mod 4 = 0 ->
+    initialL.(getLog) = [] ->
+    machine_ok p_functions main_relative_pos stack_start stack_pastend binary p_call
+               p_call mH Rdata Rexec mmioRange initialL ->
+    (scalar (word.of_Z input_ptr) input * scalar (word.of_Z output_ptr) output_placeholder * R)%sep mH ->
+    exists steps_remaining finalL mH',
+      run sched steps_remaining initialL = (Some tt, finalL) /\
+      machine_ok p_functions main_relative_pos stack_start stack_pastend binary p_call
+                 (word.add p_call (word.of_Z 4)) mH' Rdata Rexec mmioRange finalL /\
+      (scalar (word.of_Z input_ptr) input *
+       scalar (word.of_Z output_ptr) (word.add (word.of_Z 1) input) * R)%sep mH' /\
+      finalL.(getLog) = initialL.(getLog) (* no external interactions happened *).
+Proof.
+  intros.
+  change binary with (Pipeline.instrencode put_wait_get_asm).
+  refine (bedrock2_and_cava_system_correct
+            _ _ _ _ _ _ _ _ _ _ _ _ _ _ _ _ _ _ _ _ _ _ _ _ _ _ _ _ _ _ _ _ _ _);
+    try eassumption.
+  { exact funcs_valid. }
+  { apply List.dedup_NoDup_iff with (aeqb_spec:=String.eqb_spec). reflexivity. }
+  { exact put_wait_get_compile_result_eq. }
+  { (* check that the compiler emitted valid instructions: *)
+    repeat (apply Forall_cons || apply Forall_nil).
+    all: vm_compute; try intuition discriminate. }
+  { unfold main_relative_pos.
+    match goal with
+    | H: _ <= ?x < _ |- _ <= _ + ?x' < _ => change x' with x
+    end.
+    Lia.lia. }
+  { instantiate (2 := "main"). reflexivity. }
+  { reflexivity. }
+  { ZnWords. }
+  { cbn. eexists. split; [reflexivity|].
+    match goal with
+    | |- _ _ ?x => replace x with device.reset_state by case TODO
+    end.
+    (* TODO put in machine_ok, but maybe require a "ready predicate" instead of reset state,
+       and make sure that the IncrementWait program puts the device back into a ready state *)
+    exact initial_device_states_related. }
+  { refine (@WeakestPreconditionProperties.Proper_cmd _ StateMachineSemantics.ok _ _ _ _ _ _ _ _ _ _ _).
+    1: eapply WeakestPreconditionProperties.Proper_call.
+    2: {
+      eapply main_correct. 1: eassumption.
+      match goal with
+      | H: ?t = ?t' |- _ ?t'' _ => replace t'' with t' by exact H
+      end.
+      reflexivity. }
+    unfold post_main.
+    repeat intro. Tactics.logical_simplify. Tactics.ssplit. 1: eassumption.
+    do 2 eexists.
+    match goal with
+    | H: ?t = ?t' |- _ = _ ++ ?t'' /\ _ => replace t'' with t' by exact H
+    end.
+    rewrite List.app_nil_r. split; [reflexivity|]. eassumption. }
+Qed.
+
+(* Goal: bring this list down to only standard axioms like functional and propositional extensionality
+Print Assumptions IncrementWait_end2end_correct.
+*)
